@prefix audit: <https://data.archiefpunt.be/_audit/> .
@prefix owl: <http://www.w3.org/2002/07/owl#> .
@prefix rdf: <http://www.w3.org/1999/02/22-rdf-syntax-ns#> .
@prefix rdfs: <http://www.w3.org/2000/01/rdf-schema#> .
@prefix xsd: <http://www.w3.org/2001/XMLSchema#> .

audit: a owl:Ontology;
  <dc11:creator> "LIBIS";
  <dc11:date> "2022-08-30 15:37:15 +0200";
  <dc11:description> "";
  <dc11:title> "AUDIT ontology";
  owl:versionInfo 0.2 .

audit:change_reason a rdf:Property;
  rdfs:label "change_reason";
  rdfs:comment "a short, human readable description of the purpose for the changeset";
  rdfs:domain audit:ChangeSet;
  rdfs:range xsd:string .

audit:created_date a rdf:Property;
  rdfs:label "created_date";
  rdfs:comment "the date that the changeset was created. The date should be in W3CDTF format ";
  rdfs:domain audit:ChangeSet;
  rdfs:range xsd:dateTime .

audit:creator_group a rdf:Property;
  rdfs:label "creator_group";
  rdfs:comment "the name of the group responsible for creating the changeset";
  rdfs:domain audit:ChangeSet;
  rdfs:range xsd:string .

audit:creator_name a rdf:Property;
  rdfs:label "creator_name";
  rdfs:comment "the name of the entity responsible for creating the changeset";
  rdfs:domain audit:ChangeSet;
  rdfs:range xsd:string .

audit:other_data a rdf:Property;
  rdfs:label "other_data";
  rdfs:comment "data pushed from the enduser";
  rdfs:domain audit:ChangeSet;
  rdfs:range rdf:JSON .

audit:preceding_change_set a rdf:Property;
  rdfs:label "preceding_change_set";
  rdfs:comment "This property can be used to build a history of changes to a particular resource description";
  rdfs:domain audit:ChangeSet;
  rdfs:range audit:ChangeSet .

audit:subject_of_change a rdf:Property;
  rdfs:label "subject_of_change";
  rdfs:comment "the resource to which this set of changes applies";
  rdfs:domain audit:ChangeSet;
  rdfs:range xsd:anyURI .

audit:diff a rdf:Property;
  rdfs:label "diff";
  rdfs:comment "changes in hashdiff format";
  rdfs:domain audit:ChangeSet;
  rdfs:range rdf:JSON .

audit:id a rdf:Property;
  rdfs:label "id";
  rdfs:comment "uuid";
  rdfs:domain audit:ChangeSet;
  rdfs:range xsd:string .

audit:ChangeSet a owl:Class;
  rdfs:label "ChangeSet";
  rdfs:comment "The encapsulation of a delta between two versions of a resource description";
  rdfs:subClassOf [
    a owl:Restriction;
    owl:minCardinality 1;
    owl:onProperty audit:id
  ], [
    a owl:Restriction;
    owl:maxCardinality 1;
    owl:onProperty audit:id
  ], [
    a owl:Restriction;
    owl:minCardinality 1;
    owl:onProperty audit:diff
  ], [
    a owl:Restriction;
    owl:maxCardinality 1;
    owl:onProperty audit:diff
  ], [
    a owl:Restriction;
    owl:maxCardinality 1;
    owl:onProperty audit:subject_of_change
  ], [
    a owl:Restriction;
    owl:maxCardinality 1;
    owl:onProperty audit:preceding_change_set
  ], [
    a owl:Restriction;
    owl:maxCardinality 1;
    owl:onProperty audit:created_date
  ], [
    a owl:Restriction;
    owl:maxCardinality 1;
    owl:onProperty audit:change_reason
  ], [
    a owl:Restriction;
    owl:maxCardinality 1;
    owl:onProperty audit:creator_name
  ], [
    a owl:Restriction;
    owl:maxCardinality 1;
    owl:onProperty audit:creator_group
  ], [
    a owl:Restriction;
    owl:maxCardinality 1;
    owl:onProperty audit:other_data
  ] .
